

# Sequences and Limits

### 1

$$
a_n=\frac{2n^2+3n-1}{5n^2-n+2}\quad\Rightarrow\quad 
\lim_{n\to\infty}a_n=\frac{2}{5}.
$$

**Idea**: Ratio of the leading coefficients of the highest-degree terms.

---

### 2

$$
b_n=\Bigl(1+\frac1n\Bigr)^n\quad\Rightarrow\quad 
\lim_{n\to\infty}b_n=e.
$$

**Idea**: Classical definition of \$e\$.

---

### 3

$$
c_n=\frac{(-1)^n n}{n+1}=(-1)^n\cdot\frac{n}{n+1}.
$$

As \$n\to\infty\$, \$\frac{n}{n+1}\to1\$, but since \$(-1)^n\$ oscillates, even terms approach \$1\$ while odd terms approach \$-1\$.
**Conclusion**: Divergent (two subsequences have different limits).

---

### 4

$$
d_n=\frac{n!}{n^n}.
$$

Using Stirling’s formula \$n!\sim \sqrt{2\pi n},(n/e)^n\$:

$$
d_n\sim \sqrt{2\pi n}\,e^{-n}\xrightarrow[n\to\infty]{}0.
$$

**Conclusion**: \$\lim d\_n=0\$.
(Alternatively, by AM–GM or squeeze, one can get an upper bound of order \$(1/e)^n\$.)

---

### 5

$$
e_n=\frac{\sqrt{n^2+3n}-n}{n}
=\frac{3n}{n\bigl(\sqrt{n^2+3n}+n\bigr)}
=\frac{3}{\sqrt{n^2+3n}+n}\xrightarrow[n\to\infty]{}0.
$$

**Idea**: Multiply by the conjugate, denominator \$\sim 2n\$.

---

### 6

$$
f_n=\sum_{k=1}^n \frac{1}{k^2}.
$$

Each term is positive, so \$f\_n\$ is **monotonically increasing**. By comparison with an integral or using a known result, \$\sum 1/k^2\$ **converges**, and the limit is

$$
\sum_{k=1}^{\infty}\frac{1}{k^2}=\frac{\pi^2}{6}\approx1.644934.
$$

**Conclusion**: Monotonically increasing and bounded above (e.g., by \$\pi^2/6\$), hence convergent, with the limit above.

---

### 7

$$
g_n=\frac{n^3+2n}{\sqrt{n^6+n^2+1}}
=\frac{n^3\bigl(1+\frac{2}{n^2}\bigr)}{n^3\sqrt{1+\frac{1}{n^4}+\frac{1}{n^6}}}
\longrightarrow \frac{1}{1}=1.
$$

**Conclusion**: \$\lim g\_n=1\$.

---

### 8

$$
h_n=\Bigl(\frac{n}{n+1}\Bigr)^{n^2}=\bigl(1-\tfrac{1}{n+1}\bigr)^{n^2}.
$$

Take logarithm: \$\ln h\_n=n^2\ln\bigl(1-\frac{1}{n+1}\bigr)\sim n^2\cdot\bigl(-\frac{1}{n+1}\bigr)\sim -n\to-\infty\$.
**Conclusion**: \$\lim h\_n=0\$.

---

### 9

$$
i_n=n\bigl(\sqrt{n+1}-\sqrt{n}\bigr)
=n\cdot\frac{1}{\sqrt{n+1}+\sqrt{n}}
\sim \frac{n}{2\sqrt{n}}=\frac{\sqrt{n}}{2}\xrightarrow[n\to\infty]{}+\infty.
$$

**Conclusion**: Diverges to \$+\infty\$.

---

### 10

$$
j_n=\frac{a^n+b^n}{c^n+d^n},\quad a,b,c,d>0,\ a\le b,\ c\le d.
$$

* **(a) If \$b\<d\$**: Denominator dominates, \$\displaystyle \lim j\_n=0\$.
* **(b) If \$b=d\$**:
  $j_n=\frac{b^n\bigl((a/b)^n+1\bigr)}{b^n\bigl((c/b)^n+1\bigr)}\to \frac{0+1}{0+1}=1.$
* **(c) If \$b>d\$**: Numerator dominates, \$\displaystyle j\_n\sim \bigl(\frac{b}{d}\bigr)^n\to+\infty\$.

---


